code/ecdsap256sha2/Hacl.Impl.ECDSA.P256SHA256.Signature.fst
@@ -47,8 +47,7 @@ val ecdsa_signature_step12: alg: hash_alg {SHA2_256? alg \/ SHA2_384? alg \/ SHA
     (
       assert_norm (pow2 32 < pow2 61);
       assert_norm (pow2 32 < pow2 125);
-      let hashFun = hashSpec alg in 
-      let hashM = hashFun (as_seq h0 m) in 
+      let hashM = (hashSpec alg) (as_seq h0 m) in 
       let cutHashM = Lib.Sequence.sub hashM 0 32 in 
       as_nat h1 result = nat_from_bytes_be cutHashM % prime_p256_order
     )
@@ -195,7 +194,7 @@ let ecdsa_signature_step6 result kFelem z r da =
       lemma_mod_mul_distr_r br0 br1 prime_p256_order
 
 
-val ecdsa_signature_core: alg: hash_alg -> r: felem -> s: felem -> mLen: size_t -> m: lbuffer uint8 mLen ->  
+val ecdsa_signature_core: alg: hash_alg {SHA2_256? alg \/ SHA2_384? alg \/ SHA2_512? alg}  -> r: felem -> s: felem -> mLen: size_t -> m: lbuffer uint8 mLen ->  
   privKeyAsFelem: felem  -> 
   k: lbuffer uint8 (size 32) -> 
   Stack uint64
@@ -213,8 +212,10 @@ val ecdsa_signature_core: alg: hash_alg -> r: felem -> s: felem -> mLen: size_t 
     modifies (loc r |+| loc s) h0 h1 /\
     (
       assert_norm (pow2 32 < pow2 61); 
-      let hashM = H.hash Def.SHA2_256 (as_seq h0 m) in 
-      let z = nat_from_bytes_be hashM % prime_p256_order in 
+      assert_norm (pow2 32 < pow2 125);
+      let hashM = (hashSpec alg) (as_seq h0 m) in 
+      let cutHashM = Lib.Sequence.sub hashM 0 32 in 
+      let z =  nat_from_bytes_be cutHashM % prime_p256_order in 
       let (rxN, ryN, rzN), _ = montgomery_ladder_spec (as_seq h0 k) ((0,0,0), basePoint) in 
       let (xN, _, _) = _norm (rxN, ryN, rzN) in 
       
@@ -237,7 +238,7 @@ let ecdsa_signature_core alg r s mLen m privKeyAsFelem k =
   let tempBuffer = create (size 100) (u64 0) in 
   let kAsFelem = create (size 4) (u64 0) in 
   toUint64ChangeEndian k kAsFelem;
-  ecdsa_signature_step12 alg hashAsFelem mLen m;
+  ecdsa_signature_step12 alg mLen m hashAsFelem;
   let h1 = ST.get() in 
   lemma_core_0 kAsFelem h1;
   Spec.ECDSA.changeEndianLemma (uints_from_bytes_be (as_seq h0 k));
@@ -251,7 +252,7 @@ let ecdsa_signature_core alg r s mLen m privKeyAsFelem k =
   logor step5Flag sIsZero
 
 
-val ecdsa_signature: alg: hash_alg -> result: lbuffer uint8 (size 64) -> mLen: size_t -> m: lbuffer uint8 mLen ->
+val ecdsa_signature: alg: hash_alg {SHA2_256? alg \/ SHA2_384? alg \/ SHA2_512? alg} -> result: lbuffer uint8 (size 64) -> mLen: size_t -> m: lbuffer uint8 mLen ->
   privKey: lbuffer uint8 (size 32) -> 
   k: lbuffer uint8 (size 32) -> 
   Stack uint64
@@ -268,7 +269,7 @@ val ecdsa_signature: alg: hash_alg -> result: lbuffer uint8 (size 64) -> mLen: s
      (assert_norm (pow2 32 < pow2 61);
       let resultR = gsub result (size 0) (size 32) in 
       let resultS = gsub result (size 32) (size 32) in 
-      let r, s, flagSpec = Spec.ECDSA.ecdsa_signature (uint_v mLen) (as_seq h0 m) (as_seq h0 privKey) (as_seq h0 k) in 
+      let r, s, flagSpec = Spec.ECDSA.ecdsa_signature alg (uint_v mLen) (as_seq h0 m) (as_seq h0 privKey) (as_seq h0 k) in 
       as_seq h1 resultR == nat_to_bytes_be 32 r /\
       as_seq h1 resultS == nat_to_bytes_be 32 s /\
       flag == flagSpec 
@@ -310,5 +311,5 @@ let ecdsa_signature alg result mLen m privKey k =
   Spec.ECDSA.changeEndian_le_be (as_nat h2 r);
   Spec.ECDSA.changeEndian_le_be (as_nat h2 s);
 
-  pop_frame(); 
+  pop_frame();
   flag  
