code/ecdsap256sha2/Hacl.Impl.ECDSA.fsti
@@ -16,6 +16,7 @@ open Hacl.Hash.SHA2
 open Spec.P256
 open Spec.P256.Lemmas
 open Spec.P256.Definitions
+open Spec.Hash.Definitions
 
 open Spec.ECDSAP256.Definition
 
@@ -52,7 +53,7 @@ val ecdsa_p256_sha2_sign: result: lbuffer uint8 (size 64) -> mLen: size_t -> m: 
      (assert_norm (pow2 32 < pow2 61);
       let resultR = gsub result (size 0) (size 32) in 
       let resultS = gsub result (size 32) (size 32) in 
-      let r, s, flagSpec = Spec.ECDSA.ecdsa_signature (uint_v mLen) (as_seq h0 m) (as_seq h0 privKey) (as_seq h0 k) in 
+      let r, s, flagSpec = Spec.ECDSA.ecdsa_signature SHA2_256 (uint_v mLen) (as_seq h0 m) (as_seq h0 privKey) (as_seq h0 k) in 
       as_seq h1 resultR == nat_to_bytes_be 32 r /\
       as_seq h1 resultS == nat_to_bytes_be 32 s /\
       flag == flagSpec 
@@ -77,7 +78,7 @@ val ecdsa_p256_sha2_384_sign: result: lbuffer uint8 (size 64) -> mLen: size_t ->
      (assert_norm (pow2 32 < pow2 61);
       let resultR = gsub result (size 0) (size 32) in 
       let resultS = gsub result (size 32) (size 32) in 
-      let r, s, flagSpec = Spec.ECDSA.ecdsa_signature (uint_v mLen) (as_seq h0 m) (as_seq h0 privKey) (as_seq h0 k) in 
+      let r, s, flagSpec = Spec.ECDSA.ecdsa_signature SHA2_384 (uint_v mLen) (as_seq h0 m) (as_seq h0 privKey) (as_seq h0 k) in 
       as_seq h1 resultR == nat_to_bytes_be 32 r /\
       as_seq h1 resultS == nat_to_bytes_be 32 s /\
       flag == flagSpec 
@@ -102,7 +103,7 @@ val ecdsa_p256_sha2_512_sign: result: lbuffer uint8 (size 64) -> mLen: size_t ->
      (assert_norm (pow2 32 < pow2 61);
       let resultR = gsub result (size 0) (size 32) in 
       let resultS = gsub result (size 32) (size 32) in 
-      let r, s, flagSpec = Spec.ECDSA.ecdsa_signature (uint_v mLen) (as_seq h0 m) (as_seq h0 privKey) (as_seq h0 k) in 
+      let r, s, flagSpec = Spec.ECDSA.ecdsa_signature SHA2_512 (uint_v mLen) (as_seq h0 m) (as_seq h0 privKey) (as_seq h0 k) in 
       as_seq h1 resultR == nat_to_bytes_be 32 r /\
       as_seq h1 resultS == nat_to_bytes_be 32 s /\
       flag == flagSpec 
